Add groupByRetentive spec 4 and fill in some sorries

Table/BuiltinExtensions.lean
@@ -13,6 +13,8 @@ inductive List.Sublist {α} : List α → List α → Prop
 | cons (xs ys x) : Sublist xs ys → Sublist xs (x :: ys)
 | cons2 (xs ys x) : Sublist xs ys → Sublist (x :: xs) (x :: ys)
 
+infix:65    " <+ " => List.Sublist
+
 -- TODO: could solve schema woes...
 -- mutual 
 --   inductive UniqueList (α : Type _)
@@ -806,6 +808,11 @@ theorem Decidable.prop_eq_of_decide_eq (p q : Prop)
        apply Subsingleton.helim
        rfl
 
+/-
+Takes a list `kvs` consisting of (key, value) pairs and a key `k` and returns
+a tuple `(vs, kvs')` where `vs` are all values having key `k` and `kvs'` is the
+sublist of `kvs` with key entries not equal to `k`.
+-/
 def List.matchKey {κ ν} [DecidableEq κ]
     : List (κ × ν) → κ → List ν × List (κ × ν)
 | [], _ => ([], [])
@@ -854,22 +861,25 @@ by intros xs k
        rw [Nat.add_assoc, Nat.add_comm 1, ←Nat.add_assoc]
        apply congrArg (·+1) ih
 
-theorem List.matchKey_snd_keys_neq_k_map [DecidableEq κ] (xs : List (κ × ν)) :
-  ∀ e, e ∈ (List.map Prod.fst (matchKey xs k).snd) → e ≠ k :=
-by intros e hsnd
-   induction xs with
-   | nil => cases hsnd
-   | cons x xs ih =>
-     cases Decidable.em (x.1 = k) with
-     | inl heq =>
-       apply ih
-       simp only [matchKey, heq, ite_true] at hsnd
-       exact hsnd
-     | inr hneq =>
-       simp only [matchKey, hneq, ite_false] at hsnd
-       cases hsnd with
-       | head => exact hneq
-       | tail _ hin => exact ih hin
+theorem List.not_mem_matchKey_self_map_snd {κ ν} [DecidableEq κ]
+  (k : κ) (kvs : List (κ × ν)) :
+  k ∉ map Prod.fst (matchKey kvs k).snd := by
+  intro hneg
+  induction kvs with
+  | nil => cases hneg
+  | cons kv kvs ih =>
+    apply ih
+    simp only [matchKey] at hneg
+    cases Decidable.em (kv.fst = k) with
+    | inl heq =>
+      simp only [heq, ite_true] at hneg
+      assumption
+    | inr hneq =>
+      simp only [hneq, ite_false] at hneg
+      simp only [map] at hneg
+      cases hneg with
+      | head => exact absurd rfl hneq
+      | tail _ h => exact h
 
 theorem List.fst_mem_of_pair_mem : ∀ (x : α) (y : β) (ps : List (α × β)),
   (x, y) ∈ ps → x ∈ (map Prod.fst ps)
@@ -878,9 +888,9 @@ theorem List.fst_mem_of_pair_mem : ∀ (x : α) (y : β) (ps : List (α × β)),
 | x, y, _ :: ps, List.Mem.tail a h => Mem.tail _ $ fst_mem_of_pair_mem x y ps h
 
 theorem List.matchKey_snd_keys_neq_k [DecidableEq κ] (xs : List (κ × ν)) :
-  ∀ e, e ∈ (matchKey xs k).snd → e.fst ≠ k := λ e he =>
-matchKey_snd_keys_neq_k_map xs e.fst
-  (List.fst_mem_of_pair_mem e.1 e.2 (matchKey xs k).snd he)
+  ∀ e, e ∈ (matchKey xs k).snd → e.fst ≠ k := λ e he hneg =>
+  absurd (List.fst_mem_of_pair_mem e.1 e.2 (matchKey xs k).snd he)
+         (hneg ▸ not_mem_matchKey_self_map_snd k xs)
 
 -- TODO: should we use `List.eraseDups` instead? (Uses BEq instead of DEq.)
 def List.uniqueAux {α} [DecidableEq α] : List α → List α → List α
@@ -908,6 +918,38 @@ theorem List.mem_append_front :
 | x, x' :: xs, ys, List.Mem.tail _ h =>
   List.Mem.tail x' (mem_append_front x xs ys h)
 
+theorem Or.assoc : (P ∨ Q) ∨ R ↔ P ∨ Q ∨ R :=
+  Iff.intro (λ h => h.elim (λ hpq => hpq.elim Or.inl (Or.inr ∘ Or.inl))
+                           (Or.inr ∘ Or.inr))
+            (λ h => h.elim (Or.inl ∘ Or.inl)
+                           (λ hqr => hqr.elim (Or.inl ∘ Or.inr) Or.inr))
+theorem Or.comm : P ∨ Q ↔ Q ∨ P :=
+  let flip : ∀ {R S}, R ∨ S → S ∨ R := (λ h => h.elim Or.inr Or.inl)
+  Iff.intro flip flip
+
+-- Taken from Lean 3 mathlib lib/lean/library/init/data/list/lemmas.lean 112
+theorem List.mem_append : ∀ {xs ys : List α} {a : α}, a ∈ xs ++ ys ↔ a ∈ xs ∨ a ∈ ys
+| [], ys, a => Iff.intro Or.inr (λ h => h.elim (λ h' => nomatch h') id)
+| x :: xs, ys, a =>
+  have ih := mem_append (xs := xs) (ys := ys) (a := a)
+  Iff.intro
+    (λ h => match h with
+            | .head .(x) _ => Or.inl $ Mem.head _ _
+            | .tail _ htail =>
+              match ih.mp htail with
+              | .inl hxs => Or.inl $ Mem.tail _ hxs
+              | .inr hys => Or.inr hys)
+    (λ h => match h with
+            | .inl (Mem.head _ _) => Mem.head _ _
+            | .inl (Mem.tail _ htail) => Mem.tail _ $ ih.mpr (Or.inl htail)
+            | .inr hys => Mem.tail _ $ ih.mpr (Or.inr hys))
+
+theorem List.mem_append_comm {v : α} {xs ys : List α} :
+  v ∈ xs ++ ys ↔ v ∈ ys ++ xs :=
+let flip : ∀ {as bs}, v ∈ as ++ bs → v ∈ bs ++ as :=
+  (λ h => h |> mem_append.mp |> Or.comm.mp |> mem_append.mpr)
+Iff.intro flip flip
+
 theorem List.mem_reverse_iff (x : α) (xs : List α) :
   x ∈ xs ↔ x ∈ reverse xs := by
   rw [reverse_eq_reverseSpec]
@@ -925,12 +967,16 @@ theorem List.mem_reverse_iff (x : α) (xs : List α) :
     | nil => contradiction
     | cons y ys ih =>
       simp only [reverseSpec] at hb
-      admit      
+      rw [List.mem_append_comm] at hb
+      simp only [HAppend.hAppend, Append.append, List.append] at hb
+      cases hb with
+      | head => exact Mem.head _ _
+      | tail _ htail => exact Mem.tail _ (ih htail)
 
-theorem List.unique_eq_uniqueFold_aux [DecidableEq α] :
-  ∀ (xs : List α) (acc : List α),
-  uniqueAux xs acc =
-    foldl (λ acc x => if x ∈ acc then acc else acc ++ [x]) (reverse acc) xs := sorry
+-- theorem List.unique_eq_uniqueFold_aux [DecidableEq α] :
+--   ∀ (xs : List α) (acc : List α),
+--   uniqueAux xs acc =
+--     foldl (λ acc x => if x ∈ acc then acc else acc ++ [x]) (reverse acc) xs := sorry
   --   by
   -- intros xs acc
   -- induction xs generalizing acc with
@@ -947,18 +993,18 @@ theorem List.unique_eq_uniqueFold_aux [DecidableEq α] :
   --              if x ∈ acc then reverse acc else reverse acc ++ [x] := by rw [mem_reverse_iff]
       
 
-theorem List.unique_eq_uniqueFold [DecidableEq α] :
-  ∀ (xs : List α), unique xs = uniqueFoldl xs := by
-  intros xs
-  induction xs with
-  | nil => simp [unique, uniqueFoldl, uniqueAux, foldl]
-  | cons x xs ih =>
-    simp only [unique, uniqueFoldl, uniqueAux]
-    simp only [List.not_mem_nil, ite_false]
-    rw [unique_eq_uniqueFold_aux]
-    simp only [foldl]
-    apply congrArg
-    rfl
+-- theorem List.unique_eq_uniqueFold [DecidableEq α] :
+--   ∀ (xs : List α), unique xs = uniqueFoldl xs := by
+--   intros xs
+--   induction xs with
+--   | nil => simp [unique, uniqueFoldl, uniqueAux, foldl]
+--   | cons x xs ih =>
+--     simp only [unique, uniqueFoldl, uniqueAux]
+--     simp only [List.not_mem_nil, ite_false]
+--     rw [unique_eq_uniqueFold_aux]
+--     simp only [foldl]
+--     apply congrArg
+--     rfl
 
 theorem List.all_pred {p : α → Prop} [DecidablePred p] {xs : List α} :
   xs.all (λ x => decide (p x)) ↔ ∀ x, x ∈ xs → p x := by
@@ -1049,9 +1095,10 @@ theorem List.uniqueAux_acc_append_filter {α} [DecidableEq α] :
   uniqueAux xs acc = reverse acc ++ unique (xs.filter (· ∉ acc))
 | [], acc => by simp [uniqueAux, reverse, reverseAux, unique]
 | x :: xs, acc =>
-  have hterm : length (filter (λ a => !decide (a ∈ acc)) xs)
+  have hterm : length (filter (λ a => decide ¬(a ∈ acc)) xs)
                 < Nat.succ (length xs) :=
     Nat.lt_of_le_of_lt (m := length xs) (filter_length _ _) (Nat.lt.base _)
+  have hterm' : length xs < (length xs).succ := Nat.le.refl
   have ih₁ := uniqueAux_acc_append_filter xs acc
   have ih₂ := uniqueAux_acc_append_filter xs (x :: acc)
   have ih₃ :=
@@ -1097,6 +1144,7 @@ theorem List.uniqueAux_acc_append_filter {α} [DecidableEq α] :
       apply Decidable.prop_eq_of_decide_eq
       rw [h_mem_iff_neg, not_or_distrib, And.comm]
 termination_by uniqueAux_acc_append_filter xs ac => xs.length
+decreasing_by assumption
 
 theorem List.uniqueAux_acc_append {α} [DecidableEq α] (xs : List α)
   (acc : List α) (h : ∀ x, x ∈ xs → ¬ (x ∈ acc)) :
@@ -1164,11 +1212,16 @@ by intros xs k
       --  rw [h_filterAux]
       --  simp only [List.map]
 
+theorem List.matchKey_length_lt {κ} [DecidableEq κ] {ν}
+                                (k : κ) (kvs : List (κ × ν)) :
+  (matchKey kvs k).2.length < kvs.length.succ :=
+  Nat.lt_of_succ_le $ Nat.succ_le_succ $ matchKey_snd_length kvs k
+
 def List.groupByKey {κ} [DecidableEq κ] {ν} : List (κ × ν) → List (κ × List ν)
 | [] => []
 | (k, v) :: kvs =>
   have h_help : (matchKey kvs k).2.length < kvs.length.succ :=
-    Nat.lt_of_succ_le $ Nat.succ_le_succ $ matchKey_snd_length kvs k
+    matchKey_length_lt k kvs
   
   let fms := matchKey kvs k
   (k, v :: fms.1) :: groupByKey fms.2
@@ -1243,10 +1296,335 @@ theorem List.length_groupByKey {κ} [DecidableEq κ] {ν} :
   apply List.length_uniqueAux (acc := [k])
   intro x
   rw [mem_singleton_iff]
-  apply matchKey_snd_keys_neq_k_map (k := k) xs
+  intro hmem hneg
+  have := not_mem_matchKey_self_map_snd x xs
+  rw [←hneg] at hmem
+  exact this hmem
 termination_by length_groupByKey xs => length xs
 decreasing_by assumption
--- END `groupByKey`
+-- END `groupByKey` - `groupBy` spec 4
+-- BEGIN `groupByRetentive` spec 4 (this might simplify some stuff above?)
+
+def Function.injective (f : α → β) := ∀ {x y}, f x = f y → x = y
+def Function.biInjective (f : α → β → γ) := ∀ x₁ x₂ y₁ y₂, 
+  f x₁ x₂ = f y₁ y₂ → x₁ = y₁ ∧ x₂ = y₂
+
+theorem List.matchKey_snd_sublist [DecidableEq κ] :
+  ∀ (k : κ) (kvs : List (κ × ν)), (matchKey kvs k).snd <+ kvs
+| _, [] => Sublist.nil
+| k, (kv :: kvs) =>
+  have ih := matchKey_snd_sublist k kvs
+  if h : kv.fst = k
+  then by simp only [matchKey, h, ite_true]; exact Sublist.cons _ _ _ ih
+  else by simp only [matchKey, h, ite_true]; exact Sublist.cons2 _ _ _ ih
+
+theorem List.matchKey_snd_sublist_of_sublist [DecidableEq κ] :
+  ∀ (k : κ) (xs ys : List (κ × ν)),
+  xs <+ ys → (matchKey xs k).snd <+ (matchKey ys k).snd := by
+  intro k xs ys h
+  induction h with
+  | nil => constructor
+  | cons xs' ys' x' h' ih =>
+    simp only [matchKey]
+    cases Decidable.em (x'.fst = k) with
+    | inl heq => simp only [heq, ite_true]; apply ih
+    | inr hneq => simp only [hneq, ite_false]; apply Sublist.cons _ _ _ ih
+  | cons2 xs' ys' x' h' ih =>
+    simp only [matchKey]
+    cases Decidable.em (x'.fst = k) with
+    | inl heq => simp only [heq, ite_true]; assumption
+    | inr hneq =>
+      simp only [hneq, ite_false]
+      apply Sublist.cons2 _ _ _ ih
+
+theorem List.mem_of_mem_sublist {xs ys : List α} {x : α} :
+  xs <+ ys → x ∈ xs → x ∈ ys
+| .cons _ _ x' hsub, hmem => Mem.tail x' (mem_of_mem_sublist hsub hmem)
+| .cons2 _ ys _ _, Mem.head _ _ => Mem.head x ys
+| .cons2 _ _ _ hsub, Mem.tail _ hmem =>
+  Mem.tail _ (mem_of_mem_sublist hsub hmem)
+
+theorem List.fst_groupByKey_sublist [DecidableEq κ] : ∀ (kvs : List (κ × ν)),
+  map Prod.fst (groupByKey kvs) <+ map Prod.fst kvs
+| [] => Sublist.nil
+| (k, v) :: kvs =>
+  have hterm := matchKey_length_lt k kvs
+  have ih := fst_groupByKey_sublist (matchKey kvs k).snd
+  have hsubl := matchKey_snd_sublist k kvs
+  Sublist.cons2 _ _ _ $
+    Sublist.trans ih (sublist_of_map_sublist _ _ _ hsubl)
+termination_by fst_groupByKey_sublist kvs => kvs.length
+decreasing_by assumption
+
+-- It would be nice to do this fully in tactic mode, but there doesn't seem to
+-- be a way to retain unused `have`s as termination hints in tactic mode
+theorem List.mem_fst_matchKey_key_or_snd [DecidableEq κ]
+  {ys : List (κ × ν)} {x : κ} :
+  x ∈ map Prod.fst ys → ∀ k, x = k ∨ x ∈ map Prod.fst (matchKey ys k).snd :=
+λ hx k =>
+  if h : x = k
+  then Or.inl h
+  else Or.inr $
+    match ys with
+    | (k', v) :: ys =>
+      have h_term : length (matchKey ys k).snd < Nat.succ (length ys) :=
+        matchKey_length_lt k ys
+      have h_term' : length ys < Nat.succ (length ys) := Nat.le.refl
+      by
+      simp only [matchKey]
+      cases Decidable.em (k' = k) with
+      | inl hkeq =>
+        simp only [hkeq, ite_true]
+        have : x ∈ map Prod.fst ys := by
+          cases hx with
+          | head => contradiction
+          | tail => assumption
+        have ih := mem_fst_matchKey_key_or_snd this k
+        cases ih with
+        | inl => contradiction
+        | inr hmem => exact hmem
+      | inr hkneq =>
+        simp only [hkneq, ite_false]
+        simp only [groupByKey]
+        simp only [map]
+        cases Decidable.em (x = k') with
+        | inl hxeq => rw [hxeq]; apply Mem.head
+        | inr hxneq =>
+          apply Mem.tail
+          have : x ∈ map Prod.fst (matchKey ys k).snd := by
+            cases hx with
+            | head => contradiction
+            | tail _ htail => 
+              have := mem_fst_matchKey_key_or_snd htail k
+              cases this with
+              | inl => contradiction
+              | inr => assumption
+          have ih := mem_fst_matchKey_key_or_snd this k'
+          cases ih with
+          | inl => contradiction
+          | inr => assumption
+termination_by mem_fst_matchKey_key_or_snd ys x hx k => ys.length
+decreasing_by assumption
+
+-- TODO: avoid copy/paste?
+theorem List.mem_fst_groupByKey_key_or_snd [DecidableEq κ]
+  {ys : List (κ × ν)} {x : κ} :
+  x ∈ map Prod.fst ys →
+    ∀ k, x = k ∨ x ∈ map Prod.fst (groupByKey (matchKey ys k).snd) :=
+λ hx k =>
+  if h : x = k
+  then Or.inl h
+  else Or.inr $
+    match ys with
+    | (k', v) :: ys =>
+      have h_term : length (matchKey ys k).snd < Nat.succ (length ys) :=
+        matchKey_length_lt k ys
+      have h_term' : length ys < Nat.succ (length ys) := Nat.le.refl
+      by
+      simp only [matchKey]
+      cases Decidable.em (k' = k) with
+      | inl hkeq =>
+        simp only [hkeq, ite_true]
+        have : x ∈ map Prod.fst ys := by
+          cases hx with
+          | head => contradiction
+          | tail => assumption
+        have ih := mem_fst_groupByKey_key_or_snd this k
+        cases ih with
+        | inl => contradiction
+        | inr hmem => exact hmem
+      | inr hkneq =>
+        simp only [hkneq, ite_false]
+        simp only [groupByKey]
+        simp only [map]
+        cases Decidable.em (x = k') with
+        | inl hxeq => rw [hxeq]; apply Mem.head
+        | inr hxneq =>
+          apply Mem.tail
+          have : x ∈ map Prod.fst (matchKey ys k).snd := by
+            cases hx with
+            | head => contradiction
+            | tail _ htail => 
+              have := mem_fst_matchKey_key_or_snd htail k
+              cases this with
+              | inl => contradiction
+              | inr => assumption
+          have ih := mem_fst_groupByKey_key_or_snd this k'
+          cases ih with
+          | inl => contradiction
+          | inr => assumption
+termination_by mem_fst_groupByKey_key_or_snd ys x hx k => ys.length
+decreasing_by assumption
+
+/-
+Although tempting, the stronger claim
+  `xs <+ ys → map Prod.fst (groupByKey xs) <+ map Prod.fst (groupByKey ys)`
+does not hold, as the following counterexample illustrates:
+
+* `List.groupByKey [("a", 1), ("b", 2), ("a", 3)]`
+* `List.groupByKey [("b", 2), ("a", 3)]`
+
+Also, the initial hypothesis is a bit stricter than it needs to be:
+`(∀ x, x ∈ xs → x ∈ ys)` would suffice.
+-/
+
+theorem List.all_in_map_fst_groupByKey_of_sublist [DecidableEq κ]
+  {xs ys : List (κ × ν)} :
+  xs <+ ys →
+    ∀ x, x ∈ map Prod.fst (groupByKey xs) → x ∈ map Prod.fst (groupByKey ys)
+| .cons xs ys (k, v) hsubl, x, hx =>
+  if heq : x = k
+  then heq ▸ Mem.head x (map Prod.fst (groupByKey (matchKey ys k).snd))
+  else
+    have hterm : ys.length < Nat.succ ys.length := Nat.le.refl
+    have ih := all_in_map_fst_groupByKey_of_sublist hsubl x hx
+    have hor : x = k ∨ x ∈ map Prod.fst (groupByKey (matchKey ys k).snd) :=
+      mem_fst_groupByKey_key_or_snd
+        (mem_of_mem_sublist (fst_groupByKey_sublist ys) ih) k
+    Mem.tail k $
+    match hor with
+    | .inl hxeq => absurd hxeq heq
+    | .inr hmem => hmem
+| .cons2 xs ys (k, v) hsubl, x, hx => by
+    simp only [groupByKey]
+    simp only [map]
+    simp only [groupByKey] at hx
+    simp only [map] at hx
+    cases hx with
+    | head => constructor
+    | tail _ htail =>
+      apply Mem.tail
+      have : (matchKey xs k).snd <+ (matchKey ys k).snd :=
+        matchKey_snd_sublist_of_sublist _ _ _ hsubl
+      have hterm := matchKey_length_lt k ys
+      apply all_in_map_fst_groupByKey_of_sublist this
+      assumption
+termination_by all_in_map_fst_groupByKey_of_sublist xs ys hsubl x hx =>
+  ys.length
+decreasing_by assumption
+
+-- #check @List.not_mem_matchKey_self_snd
+-- #check @List.matchKey_snd_sublist
+-- #check @List.matchKey_snd_sublist_of_sublist
+-- theorem List.map_groupByKey_matchKey_wip [DecidableEq κ] {k : κ} {kvs : List (κ × ν)} :
+--   ∀ x, x ∈ map Prod.fst (groupByKey (matchKey kvs k).snd) → x ∈ map Prod.fst (groupByKey kvs) := by
+--   intro x hx
+--   induction kvs with
+--   | nil => simp only [groupByKey, map] at hx; contradiction
+--   | cons kv kvs ih =>
+--     cases kv with | mk k' v =>
+--     -- simp only [matchKey] at hx
+--     simp only [groupByKey]
+--     simp only [map]
+--     cases Decidable.em (x = k') with
+--     | inl heq =>
+--       rw [heq]
+--       apply Mem.head
+--     | inr hneq =>
+--       simp only [matchKey] at hx
+--       apply Mem.tail
+--       cases Decidable.em (k' = k) with
+--       | inl heq' =>
+--         simp only [heq', ite_true] at hx
+--         rw [heq']
+--         apply hx
+--       | inr hneq' =>
+--         simp only [hneq', ite_false] at hx
+--         simp only [groupByKey] at hx
+--         simp only [map] at hx
+--         have := matchKey_snd_sublist k' (matchKey kvs k).snd
+--         sorry
+
+-- The converse is also true, but we don't need it here
+theorem List.mem_fsts_of_mem_fsts_groupByKey [DecidableEq κ] (kvs : List (κ × ν)) :
+  k ∈ map Prod.fst (groupByKey kvs) → k ∈ map Prod.fst kvs := by
+  intro h
+  induction kvs with
+  | nil => contradiction
+  | cons kv kvs ih =>
+    cases kv with | mk k₀ v₀ =>
+    simp only [groupByKey] at h
+    simp only [map] at h
+    simp only [map]
+    cases h with
+    | head => apply Mem.head
+    | tail _ htail =>
+      apply Mem.tail
+      apply ih
+      apply all_in_map_fst_groupByKey_of_sublist (matchKey_snd_sublist k₀ kvs)
+      assumption
+
+-- Instead of being separate, this could just be folded into
+-- `groupByKey_fsts_no_duplicates`
+theorem List.key_not_mem_fst_groupByKey_matchKey_snd [DecidableEq κ] 
+  (kvs : List (κ × ν)) (k : κ) :
+  k ∉ map Prod.fst (groupByKey (matchKey kvs k).snd) :=
+  mt (List.mem_fsts_of_mem_fsts_groupByKey (matchKey kvs k).snd)
+    (List.not_mem_matchKey_self_map_snd _ _)
+
+-- TODO: almost certainly need something more general for the induction
+theorem List.groupByKey_fsts_no_duplicates [DecidableEq κ] :
+  ∀ (kvs : List (κ × ν)), NoDuplicates $ (groupByKey kvs).map Prod.fst
+| [] => NoDuplicates.nil
+| (k, v) :: kvs =>
+  have h_help : (matchKey kvs k).2.length < kvs.length.succ :=
+    matchKey_length_lt k kvs
+
+  NoDuplicates.cons k ((groupByKey (matchKey kvs k).2).map Prod.fst)
+    (List.key_not_mem_fst_groupByKey_matchKey_snd _ _)
+    (groupByKey_fsts_no_duplicates (matchKey kvs k).2)
+termination_by groupByKey_fsts_no_duplicates xs => xs.length
+decreasing_by assumption
+
+-- This is stated in Lean 3 mathlib's mathlib/src/data/list/basic.lean, line 114
+theorem List.mem_map {f : α → β} {b : β} : ∀ {l : List α},
+  b ∈ map f l ↔ ∃ a, a ∈ l ∧ f a = b 
+| [] => Iff.intro (λ h => nomatch h) (λ h => h.elim (λ x hx => nomatch hx.left))
+| x :: xs => by
+  have ih := @mem_map α β f b xs
+  apply Iff.intro
+  . intro h
+    cases h with
+    | head =>
+      exact Exists.intro x (And.intro (List.Mem.head _ _) rfl)
+    | tail x h' =>
+      have ih_val := ih.mp h'
+      cases ih_val with | intro a ha =>
+      exact Exists.intro a (And.intro (Mem.tail _ ha.left) ha.right)
+  . intro h
+    cases h with | intro a ha =>
+    simp only [map]
+    cases ha.left with
+    | head => rw [ha.right]; constructor
+    | tail x h' =>
+      have h_in_tail := ih.mpr (Exists.intro a ⟨h', ha.right⟩)
+      exact Mem.tail _ h_in_tail
+
+-- Stated in mathlib/src/data/list/basic.lean, line 129
+theorem List.mem_map_of_mem (f : α → β) {a : α} {l : List α} (h : a ∈ l) :
+  f a ∈ map f l :=
+mem_map.mpr (Exists.intro a (And.intro h rfl))
+
+theorem List.mem_of_mem_injective_map (f : α → β) (hf : f.injective) :
+  ∀ (x : α) (xs : List α),
+  f x ∈ map f xs ↔ x ∈ xs :=
+λ _ xs => Iff.intro
+  (λ h =>
+    have ⟨_, hb⟩ := mem_map.mp h
+    have hbeqx := hf hb.right
+    Eq.subst (motive := λ a => a ∈ xs) hbeqx hb.left
+  )
+  (mem_map_of_mem _)
+
+theorem List.no_dups_map_injective
+  (f : α → β) (hf : f.injective) : ∀ (xs : List α) (hxs : NoDuplicates xs),
+  NoDuplicates $ map f xs
+| [], hxs => NoDuplicates.nil
+| x :: xs, NoDuplicates.cons _ _ hxnin hndxs =>
+  NoDuplicates.cons (f x) (map f xs)
+    (λ hneg => absurd ((mem_of_mem_injective_map f hf x xs).mp hneg) hxnin)
+    (no_dups_map_injective f hf xs hndxs)
+-- END spec 4
 
 -- `List.counts`, helper functions, and associated theorems
 -- TODO: these proofs could probably be cleaned up a lot.
