Table/Cell.lean
@@ -27,6 +27,11 @@ def rename {nm τ} : Cell (η := η) nm τ → (nm' : η) → Cell nm' τ
 | Cell.emp, nm => Cell.emp
 | Cell.val x, nm => Cell.val x
 
+theorem toOption_fromOption {nm : η} :
+  ∀ (v : Option τ), toOption (fromOption (nm := nm) v) = v
+| none => rfl
+| some x => rfl
+
 end Cell
 
 -- Decidable equality
